EtM: adding INT-CTXT modelling

examples/crypto/EtM.Ideal.fsti
@@ -3,3 +3,8 @@ module EtM.Ideal
 val ind_cpa : bool
 
 val uf_cma : b:bool{ ind_cpa ==> b}
+
+let priv = ind_cpa
+
+let ind_cpa_rest_adv = uf_cma 
+(* well typed adversaries only submit ciphertext obtained using encrypt *)
